Update ToyClient to use recently refactored and renamed types
* Change type of EncryptionContext from Option<EncryptionContext> to EncryptionContext (an empty context is represented as an empty sequence).
* Use constructors Result.{Success,Failure}, which used to be Result.{Ok,Err}.
* Skip construction from keyring, for now.
* Format according to Dafny style guide.

Code verifies and compiles with:

    $ dafny src/SDK/AlgorithmSuite.dfy src/SDK/Common.dfy src/SDK/Keyring/Defs.dfy src/StandardLibrary/UInt.dfy src/StandardLibrary/StandardLibrary.dfy
    Dafny 2.3.0.10506

    Dafny program verifier finished with 88 verified, 0 errors
    Compiled assembly into AlgorithmSuite.dll

    $ dafny src/SDK/ToyClient.dfy src/Crypto/Signature.dfy src/Crypto/RSAEncryption.dfy src/Crypto/GenBytesExtern.cs src/Crypto/EncryptionExtern.cs lib/BouncyCastle.1.8.5/lib/BouncyCastle.Crypto.dll
    Dafny 2.3.0.10506

    Dafny program verifier finished with 15 verified, 0 errors
    Compiled program written to ToyClient.cs
    Compiled assembly into ToyClient.dll

See README.md for instructions for installing BounceCastle.

src/Crypto/EncryptionExtern.cs
@@ -36,10 +36,10 @@ namespace AESEncryption {
                 byte[] c = new byte[cipher.GetOutputSize(msg.Elements.Length)];
                 var len = cipher.ProcessBytes(msg.Elements, 0, msg.Elements.Length, c, 0);
                 cipher.DoFinal(c, len);
-                return new STL.Result_Ok<byteseq>(new byteseq(c));
+                return new STL.Result_Success<byteseq>(new byteseq(c));
             }
             catch {
-                return new STL.Result_Err<byteseq>(new Dafny.Sequence<char>("aes encrypt err".ToCharArray()));
+                return new STL.Result_Failure<byteseq>(new Dafny.Sequence<char>("aes encrypt err".ToCharArray()));
             }
         }
 
@@ -51,11 +51,11 @@ namespace AESEncryption {
                 var pt = new byte[cipher.GetOutputSize(ctx.Elements.Length)];
                 var len = cipher.ProcessBytes(ctx.Elements, 0, ctx.Elements.Length, pt, 0);
                 cipher.DoFinal(pt, len);
-                return new STL.Result_Ok<byteseq>(new byteseq(pt));
+                return new STL.Result_Success<byteseq>(new byteseq(pt));
             }
             catch {
                 // TODO: distinguish BC error from unsuccessful decrypt
-                return new STL.Result_Err<byteseq>(new Dafny.Sequence<char>("aes decrypt err".ToCharArray()));
+                return new STL.Result_Failure<byteseq>(new Dafny.Sequence<char>("aes decrypt err".ToCharArray()));
 
             }
         }
