src/SDK/ToyClient.dfy
@@ -1,117 +1,102 @@
-include "CMM/Defs.dfy"
-include "CMM/DefaultCMM.dfy"
-include "Keyring/Defs.dfy"
-include "Keyring/Defs.dfy"
-include "Common.dfy"
-include "AlgorithmSuite.dfy"
 include "../StandardLibrary/StandardLibrary.dfy"
 include "../StandardLibrary/UInt.dfy"
+include "Common.dfy"
+include "CMM/Defs.dfy"
+include "AlgorithmSuite.dfy"
 include "../Crypto/AESEncryption.dfy"
-include "../Crypto/Cipher.dfy"
 
 module ToyClientDef {
-    import opened SDKDefs
-    import opened StandardLibrary
-    import opened UInt = StandardLibrary.UInt
-    import DefaultCMMDef
-    import Keyring = KeyringDefs
-    import CMM = CMMDefs
-    import Alg = AlgorithmSuite
-    import AES = AESEncryption
-    import C = Cipher
+  import opened StandardLibrary
+  import opened UInt = StandardLibrary.UInt
+  import Materials
+  import CMMDefs
+  import AlgorithmSuite
+  import AESEncryption
+  import Cipher
 
-    datatype Encryption = Encryption(ec : EncCtx, edks : seq<EDK>, ctxt : seq<uint8>)
+  datatype Encryption = Encryption(ec: Materials.EncryptionContext, edks: seq<Materials.EncryptedDataKey>, ctxt: seq<uint8>)
 
-    class ToyClient {
-        var cmm : CMM.CMM
-        ghost var Repr : set<object>
-        predicate Valid() reads this, Repr {
-            this in Repr &&
-            cmm in Repr &&
-            Repr == {this, cmm} + cmm.Repr &&
-            cmm.Valid()
+  class Client {
+    var cmm: CMMDefs.CMM
+    ghost var Repr: set<object>
+    predicate Valid()
+      reads this, Repr
+    {
+      this in Repr &&
+      cmm in Repr && cmm.Repr <= Repr && this !in cmm.Repr && cmm.Valid()
+    }
+    constructor OfCMM(c: CMMDefs.CMM) requires c.Valid() ensures Valid() {
+      cmm := c;
+      Repr := {this, cmm} + c.Repr;
+    }
+    /*
+    constructor OfKeyring(k: Keyring.Keyring) requires k.Valid() ensures Valid() ensures fresh(cmm) {
+      cmm := new DefaultCMMDef.DefaultCMM.OfKeyring(k);
+      new;
+      Repr := {this, cmm} + cmm.Repr;
+    }
+    */
+    method GetEncMaterials(ec: Materials.EncryptionContext) returns (res: Result<Materials.EncryptionMaterials>)
+      requires Valid()
+      ensures Valid()
+      ensures res.Success? ==> res.value.algorithmSuiteID == AlgorithmSuite.AES_256_GCM_IV12_TAG16_HKDF_SHA384_ECDSA_P384
+      ensures res.Success? ==> res.value.plaintextDataKey.Some?
+    {
+      var rResult := cmm.EncMatRequest(ec, None, None);
+      match rResult
+      case Failure(err) =>
+        return Failure(err);
+      case Success(r) =>
+        if r.algorithmSuiteID != AlgorithmSuite.AES_256_GCM_IV12_TAG16_HKDF_SHA384_ECDSA_P384 {
+          return Failure("bad alg id");
+        } else if r.plaintextDataKey.None? {
+          return Failure("bad data key");
         }
-        constructor OfCMM(c : CMM.CMM) requires c.Valid() ensures Valid() {
-            cmm := c;
-            new;
-            Repr := {this, cmm} + cmm.Repr;
-        } 
-        constructor OfKeyring(k : Keyring.Keyring) requires k.Valid() ensures Valid() ensures fresh(cmm) {
-            cmm := new DefaultCMMDef.DefaultCMM.OfKeyring(k);
-            new;
-            Repr := {this, cmm} + cmm.Repr;
-        } 
-        method GetEncMaterials(ec : EncCtx) returns (res : Result<EncMaterials>) requires Valid() ensures Valid()
-            ensures res.Ok? ==> res.get.alg_id == (Alg.AES_256_GCM_IV12_AUTH16_KDSHA384_SIGEC384)
-            ensures res.Ok? ==> res.get.data_key.Some?
-        {
-            res := cmm.EncMatRequest(ec, None, None);
-            if res.Ok? {
-                var r := res.get;
-                if r.alg_id != (Alg.AES_256_GCM_IV12_AUTH16_KDSHA384_SIGEC384) {
-                    res := Err("bad alg id");
-                }
-                if r.data_key.None? {
-                    res := Err("bad data key");
-                }
-            }
-            else {
-                return Err(res.err);
-            }
-        }
-
-        method Enc(pt : seq<uint8>, ec : EncCtx) returns (res : Result<(Encryption)>) requires Valid() ensures Valid()
-        {
-            var oem := GetEncMaterials(ec);
-            match oem {
-                case Ok (em) => {
-                    if |em.data_key.get| == 32 {
-                        var ctxt := AES.AES.AESEncrypt(C.AES_GCM_256, (em.data_key.get), (pt), ([]));
-                        if ctxt.Ok? {
-                            return Ok(Encryption(em.enc_ctx, em.edks, ctxt.get));
-                        }
-                        else {
-                            return Err("bad ctxt in Enc");
-                        }
-                    }
-                    else { return Err("bad data key length"); }
-
-                }
-                case Err(e) => {return Err(e);}
-            }
-        }
-
-        method Dec(e : Encryption) returns (res : Result<seq<uint8>>) requires Valid() ensures Valid()
-        {
-            if |e.edks| == 0 {
-                return Err("no edks");
-            }
-            var odecmat := cmm.DecMatRequest(Alg.AES_256_GCM_IV12_AUTH16_KDSHA384_SIGEC384, e.edks, e.ec);
-            match odecmat {
-                case Ok(decmat) => {
-                    match decmat.data_key {
-                        case Some(dk) => {
-                            if |dk| == 32 && |e.ctxt| > 12 {
-                                var msg := AES.AES.AESDecrypt(C.AES_GCM_256, (dk), ([]), (e.ctxt));
-                                return msg;
-                            }
-                            else {
-                                return Err("bad dk");
-                            }
-                        }
-                        case None => {
-                            return Err("no dk?");
-                        }
-                    }
-
-                }
-                case Err(e) => {
-                    return Err(e);
-                }
-            }
-        }
-
-
+        return Success(r);
     }
 
+    method Encrypt(pt: seq<uint8>, ec: Materials.EncryptionContext) returns (res: Result<Encryption>)
+      requires Valid()
+      ensures Valid()
+    {
+      var emResult := GetEncMaterials(ec);
+      match emResult
+      case Failure(err) =>
+        return Failure(err);
+      case Success(em) =>
+        if |em.plaintextDataKey.get| != 32 {
+          return Failure("bad data key length");
+        }
+        var ciphertextResult := AESEncryption.AES.AESEncrypt(Cipher.AES_GCM_256, em.plaintextDataKey.get, pt, []);
+        match ciphertextResult
+        case Success(ciphertext) =>
+          return Success(Encryption(em.encryptionContext, em.encryptedDataKeys, ciphertext));
+        case Failure(err) =>
+          return Failure(err);
+    }
+
+    method Decrypt(e: Encryption) returns (res: Result<seq<uint8>>)
+      requires Valid()
+      ensures Valid()
+    {
+      if |e.edks| == 0 {
+        return Failure("no edks");
+      }
+      var decmatResult := cmm.DecMatRequest(AlgorithmSuite.AES_256_GCM_IV12_TAG16_HKDF_SHA384_ECDSA_P384, e.edks, e.ec);
+      match decmatResult
+      case Failure(err) =>
+        return Failure(err);
+      case Success(decmat) =>
+        match decmat.plaintextDataKey
+        case Some(dk) =>
+          if |dk| == 32 && |e.ctxt| > 12 {
+            var msg := AESEncryption.AES.AESDecrypt(Cipher.AES_GCM_256, dk, [], e.ctxt);
+            return msg;
+          } else {
+            return Failure("bad dk");
+          }
+        case None =>
+          return Failure("no dk?");
+    }
+  }
 }
