src/SDK/CMM/Defs.dfy
@@ -3,27 +3,24 @@ include "../../StandardLibrary/StandardLibrary.dfy"
 include "../../StandardLibrary/UInt.dfy"
 
 module CMMDefs {
-    import opened SDKDefs
-    import opened StandardLibrary
-    import opened UInt = StandardLibrary.UInt
-    import AlgorithmSuite
+  import opened StandardLibrary
+  import opened UInt = StandardLibrary.UInt
+  import Materials
+  import AlgorithmSuite
 
-    trait {:termination false} CMM {
-        ghost var Repr : set<object>
-        predicate Valid() reads this, Repr
+  trait {:termination false} CMM {
+    ghost var Repr : set<object>
+    predicate Valid() reads this, Repr
 
-        method EncMatRequest(ec : EncCtx, alg_id : Option<AlgorithmSuite.ID>, pt_len : Option<nat>) returns (res : Result<EncMaterials>)
-            requires Valid()
-            ensures Valid()
-            ensures res.Ok? ==> WFEncMaterials(res.get)
+    method EncMatRequest(ec: Materials.EncryptionContext, alg_id: Option<AlgorithmSuite.ID>, pt_len: Option<nat>) returns (res: Result<Materials.EncryptionMaterials>)
+      requires Valid()
+      ensures Valid()
+      ensures res.Success? ==> res.value.Valid()
 
-        method DecMatRequest(alg_id : AlgorithmSuite.ID, edks : seq<EDK>, enc_ctx : EncCtx) returns (res : Result<DecMaterials>)
-            requires |edks| > 0
-            requires Valid()
-            ensures Valid()
-            ensures res.Ok? ==> WFDecMaterials(res.get)
-    }
-
-
-
+    method DecMatRequest(alg_id: AlgorithmSuite.ID, edks: seq<Materials.EncryptedDataKey>, enc_ctx: Materials.EncryptionContext) returns (res: Result<Materials.DecryptionMaterials>)
+      requires |edks| > 0
+      requires Valid()
+      ensures Valid()
+      ensures res.Success? ==> res.value.Valid()
+  }
 }
